examples/bintree.v
@@ -1,0 +1,252 @@
+
+From Coq Require Import ssreflect ssrbool ssrfun.
+From mathcomp Require Import eqtype seq ssrnat.
+From fcsl Require Import axioms pred.
+From fcsl Require Import pcm unionmap heap autopcm automap.
+From HTT Require Import model heapauto.
+From HTT Require Import llist.
+Set Implicit Arguments.
+Unset Strict Implicit.
+Unset Printing Implicit Defensive.
+Obligation Tactic := auto.
+
+(* Binary tree specification *)
+
+Inductive tree A := Leaf | Node of (tree A) & A & (tree A).
+
+Definition leaf {A} : tree A := @Leaf A.
+
+Fixpoint size_tree {A} (t : tree A) : nat :=
+  if t is Node l _ r
+    then (size_tree l + size_tree r).+1
+  else 0.
+
+Fixpoint inorder {A} (t : tree A) : seq A :=
+  if t is Node l x r
+    then inorder l ++ x :: inorder r
+  else [::].
+
+(* Add an element to the rightmost branch *)
+
+Fixpoint addr {A} (y : A) (t : tree A) : tree A :=
+  if t is Node l x r
+    then Node l x (addr y r)
+  else Node leaf y leaf.
+
+(* Tree heap predicate: [left branch pointer, value, right branch pointer] *)
+
+Fixpoint shape {A} (p : ptr) (t : tree A) :=
+  if t is Node l a r then
+    [Pred h | exists l' r' h',
+          h = p :-> l' \+ (p .+ 1 :-> a \+ (p .+ 2 :-> r' \+ h'))
+       /\ h' \In shape l' l # shape r' r]
+  else [Pred h | p = null /\ h = Unit].
+
+(* Null pointer represents a leaf *)
+
+Lemma shape_null {A} (t : tree A) h :
+        valid h -> h \In shape null t ->
+        t = leaf /\ h = Unit.
+Proof.
+move=>V; case: t=>/= [|l a r]; first by case=>_->.
+by case=>?[?][?][E]; rewrite E validPtUn in V.
+Qed.
+
+(* Non-null pointer represents a node *)
+
+Lemma shape_cont {A} (t : tree A) p h :
+        p != null -> h \In shape p t ->
+        exists l a r l' r' h',
+         [/\ t = Node l a r,
+             h = p :-> l' \+ (p .+ 1 :-> a \+ (p .+ 2 :-> r' \+ h'))
+           & h' \In shape l' l # shape r' r].
+Proof.
+move=>E; case: t=>/= [|l a r].
+- by case=>E0; rewrite E0 in E.
+case=>l'[r'][h'][E1 E2].
+by exists l,a,r,l',r',h'.
+Qed.
+
+Section Tree.
+Variable A : Type.
+
+(* Node creation *)
+
+Program Definition mknode (x : A) :
+  STsep (emp,
+        [vfun p => shape p (Node leaf x leaf)]) :=
+  Do (n <-- allocb null 3;
+      n.+ 1 ::= x;;
+      ret n).
+Next Obligation.
+(* the starting heap is empty *)
+move=>x [] _ /= ->.
+(* run all the steps *)
+step=>n; rewrite !unitR ptrA; step; step=>_.
+(* the postcondition is satisfied *)
+by exists null, null, Unit; vauto; rewrite unitR.
+Qed.
+
+(* Recursive tree disposal *)
+
+(* We start from a well-formed tree and arrive at an empty heap *)
+Definition disposetreeT : Type :=
+  forall p, {t : tree A}, STsep (shape p t, [vfun _ : unit => emp]).
+
+Program Definition disposetree : disposetreeT :=
+  Fix (fun (loop : disposetreeT) p =>
+       Do (if p == null then ret tt
+           else l <-- !p;
+                r <-- !(p.+ 2);
+                loop l;;
+                loop r;;
+                dealloc p;;
+                dealloc p.+ 1;;
+                dealloc p.+ 2
+                )).
+Next Obligation.
+(* pull out ghost var + precondition, branch on null check *)
+move=>loop p [t][] i /= H; case: eqP H=>[{p}->|/eqP E] H.
+- (* null pointer is an empty tree, so the heap is empty *)
+  by apply: vrfV=>V; step=>_; case: (shape_null V H).
+(* non-null pointer is a node, deconstruct it, read branch pointers *)
+case: (shape_cont E H)=>l[a][r][l'][r'][_][{t H E}_ {i}-> [hl][hr][-> Hl Hr]].
+do 2!step.
+(* recursive calls vacate left+right subheaps *)
+apply: [stepX l]@hl=>//= _ _ ->; rewrite unitL.
+apply: [stepX r]@hr=>//= _ _ ->; rewrite unitR.
+(* deallocating the node vacates the remainder *)
+by do 3!step; rewrite !unitL.
+Qed.
+
+(* Calculation of tree size *)
+
+(* loop invariant: *)
+(* the subtree size is added to the accumulator *)
+Definition treesizeT : Type := forall (ps : ptr * nat),
+  {t : tree A}, STsep (shape ps.1 t,
+                      [vfun s h => s == ps.2 + size_tree t /\ shape ps.1 t h]).
+
+Program Definition treesize p :
+  {t : tree A}, STsep (shape p t,
+                      [vfun s h => s == size_tree t /\ shape p t h]) :=
+  Do (let len := Fix (fun (go : treesizeT) '(p, s) =>
+                       Do (if p == null then ret s
+                           else l <-- !p;
+                                r <-- !(p.+ 2);
+                                ls <-- go (l, s);
+                                go (r, ls.+1)))
+      in len (p, 0)).
+Next Obligation.
+(* pull out ghost var + precondition, branch on null check *)
+move=>_ go _ p s /= _ [t][] i /= H; case: eqP H=>[{p}->|/eqP Ep] H.
+- (* empty tree has size 0 *)
+  by step=>V; case: (shape_null V H)=>->->/=; rewrite addn0.
+(* non-null pointer is a node, deconstruct it, read branch pointers *)
+  case: (shape_cont Ep H)=>l[a][r][l'][r'][_][{t H}-> {i}-> [hl][hr][-> Hl Hr]] /=.
+do 2!step.
+(* calculate left branch size, update the accumulator *)
+apply: [stepX l]@hl=>//= _ hl' [/eqP -> Hl'].
+(* add 1 to accumulator and calculate right branch size *)
+apply: [gX r]@hr=>//= _ hr' [/eqP -> Hr'] _.
+(* finish with simple arithmetic and heap manipulation *)
+by split; [rewrite addnS addSn addnA | vauto].
+Qed.
+Next Obligation.
+(* pull out ghost var + precondition, start the loop with empty accumulator *)
+by move=>/= p [t][] i /= H; apply: [gE t].
+Qed.
+
+(* Tree in-order traversal, storing the values in a linked list *)
+
+Opaque insert new.
+
+(* loop invariant: *)
+(* the subtree is unchanged, its values are prepended to the accumulator list *)
+Definition inordertravT : Type := forall (ps : ptr * ptr),
+  {(t : tree A) (l : seq A)},
+     STsep (shape ps.1 t # lseq ps.2 l,
+           [vfun s h => h \In shape ps.1 t # lseq s (inorder t ++ l)]).
+
+Program Definition inordertrav p :
+  {t : tree A}, STsep (shape p t,
+                      [vfun s h => h \In shape p t # lseq s (inorder t)]) :=
+  Do (let loop := Fix (fun (go : inordertravT) '(p, s) =>
+                       Do (if p == null then ret s
+                           else l <-- !p;
+                                a <-- !(p.+ 1);
+                                r <-- !(p.+ 2);
+                                s1 <-- go (r, s);
+                                s2 <-- insert s1 (a : A);
+                                go (l, s2)))
+      in n <-- new A;
+         loop (p, n)).
+Next Obligation.
+(* pull out ghosts + precondition, deconstruct the heap, branch on null check *)
+move=>_ go _ p s _ /= [t][xs][] _ /= [h1][h2][-> H1 H2].
+case: eqP H1=>[{p}->|/eqP Ep] H1.
+- (* return the accumulated list - empty tree has no values *)
+  by step=>V; case: (shape_null (validL V) H1)=>->->/=; vauto.
+(* non-empty tree is a node, deconstruct the node, read the pointers and the value *)
+case: (shape_cont Ep H1)=>l[a][r][l'][r'][_][{t H1}-> {h1}-> [hl][hr][-> Hl Hr]] /=.
+do 3!step.
+(* run traversal on the right branch first (it's cheaper to grow a linked list to the left) *)
+apply: [stepX r, xs]@(hr \+ h2)=>//=; first by vauto.
+(* we have subheaps corresponding to the left+right branches and the updated list *)
+move=>s1 _ [hr'][hs][-> Hr' Hs].
+(* prepend the node value to the list *)
+apply: [stepX (inorder r ++ xs)]@hs=>//= pa _ [s2][h'][-> H'].
+(* run the traversal on the left branch with updated list *)
+apply: [gX l, (a::inorder r ++ xs)]@(hl \+ pa :-> a \+ pa.+ 1 :-> s2 \+ h')=>//=.
+- (* the precondition is satisfied by simple heap manipulation *)
+  move=>_; exists hl, (pa :-> a \+ (pa.+ 1 :-> s2 \+ h')).
+  by split=>//=; [rewrite !joinA | vauto].
+(* the postcondition is also satisfied by simple massaging *)
+move=>s3 _ [hl''][hs'][-> Hl'' Hs'] _.
+exists (p :-> l' \+ (p.+ 1 :-> a \+ (p.+ 2 :-> r' \+ (hl'' \+ hr')))), hs'.
+split; try by hhauto.
+by rewrite -catA.
+Qed.
+Next Obligation.
+(* pull out ghost var + precondition *)
+move=>/= p [t][] i /= H.
+(* make an empty list by framing on Unit *)
+(* this just sets n to null, but we stick to the list API *)
+apply: [stepU]=>//= _ _ [->->]; rewrite unitL.
+(* start the loop, conditions are satisfied by simple massaging *)
+apply: [gE t, [::]]=>//=.
+- by exists i, Unit; split=>//; rewrite unitR.
+by move=>s m; rewrite cats0.
+Qed.
+
+(* Expanding the tree to the right *)
+
+Opaque mknode.
+
+(* loop invariant: the value is added to the rightmost branch *)
+Definition expandrightT x : Type := forall (p : ptr),
+  {t : tree A}, STsep (shape p t,
+                      [vfun p' => shape p' (addr x t)]).
+
+Program Definition expandright x : expandrightT x :=
+  Fix (fun (go : expandrightT x) p =>
+      Do (if p == null
+            then n <-- mknode x;
+                 ret n
+          else pr <-- !(p.+ 2);
+               p' <-- go pr;
+               p.+ 2 ::= p';;
+               ret p)).
+Next Obligation.
+(* pull out ghost + precondition, branch on null check *)
+move=>x go p [t []] i /= H; case: eqP H=>[{p}->|/eqP Ep] H.
+- (* tree is empty, make a new node and return it *)
+  apply: vrfV=>V; case: (shape_null V H)=>{t H}->{i V}->.
+  by apply: [stepE]=>//= n m H; step.
+(* tree is non-empty, i.e. a node, deconstruct it *)
+case: (shape_cont Ep H)=>l[z][r][pl][pr][_][{t H}->{i}->][hl][hr][-> Hl Hr].
+(* run the rest of the program on the right branch + subheap *)
+by step; apply: [stepX r]@hr=>//= p' h' H'; do 2!step; vauto.
+Qed.
+
+End Tree.
