examples/bst.v
@@ -1,0 +1,274 @@
+From Coq Require Import ssreflect ssrbool ssrfun.
+From mathcomp Require Import eqtype ssrnat seq path.
+From fcsl Require Import axioms pred ordtype.
+From fcsl Require Import pcm unionmap heap autopcm automap.
+From HTT Require Import interlude model heapauto.
+From HTT Require Import bintree.
+Set Implicit Arguments.
+Unset Strict Implicit.
+Unset Printing Implicit Defensive.
+Obligation Tactic := auto.
+
+Section BST.
+Context {T : ordType}.
+
+(* A binary _search_ tree remains a binary tree structurally, plus: *)
+(* 1. its elements must have an ordering defined on them            *)
+(* 2. a recursive invariant should be satisfied:                    *)
+(*    all left branch elements are smaller than the node value &    *)
+(*    all right branch elements are larger than the node value      *)
+
+(* Search tree operations *)
+
+Fixpoint insert x (t : tree T) : tree T :=
+  if t is Node l a r
+    then
+      if x == a then Node l a r
+        else if ord x a then Node (insert x l) a r
+                        else Node l a (insert x r)
+  else Node leaf x leaf.
+
+Fixpoint search (t : tree T) x : bool :=
+  if t is Node l a r
+    then
+      if x == a then true
+        else if ord x a then search l x
+                        else search r x
+  else false.
+
+(* Search tree invariant & its interaction with operations *)
+
+Fixpoint bst (t : tree T) : bool :=
+  if t is Node l a r
+    then [&& all (ord^~ a) (inorder l), all (ord a) (inorder r), bst l & bst r]
+    else true.
+
+(* Both BSTs and sorted lists can be used to implement lookup structures, but trees *)
+(* are more efficient computationally, while lists are simpler to reason about,     *)
+(* since the operations on them are associative and commute in many cases. We can   *)
+(* switch between two specification styles via the in-order traversal.              *)
+
+Lemma bst_to_sorted (t : tree T) :
+        bst t = sorted ord (inorder t).
+Proof.
+elim: t=>//=l -> a r ->.
+by rewrite sorted_cat_cons_cat /= cats1 sorted_rconsE
+  (path_sortedE (@trans T)) andbACA -andbA.
+Qed.
+
+(* An in-order specification for insertion *)
+Lemma inorder_insert x (t : tree T) :
+        bst t ->
+        perm_eq (inorder (insert x t))
+                (if x \in inorder t then inorder t else x :: inorder t).
+Proof.
+elim: t=>//=l IHl a r IHr /and4P [Hal Har /IHl Hl /IHr Hr] {IHl IHr}.
+rewrite mem_cat inE; case: (ifP [|| _, _ | _]).
+- case/or3P=>H.
+  - rewrite H in Hl.
+    move/allP: Hal=>/(_ x H) /[dup] Hxa /ord_neq/negbTE ->; rewrite Hxa /=.
+    by apply/permEl/perm_catr.
+  - by rewrite H.
+  rewrite H in Hr.
+  move/allP: Har=>/(_ x H) /[dup] /nsym/negP/negbTE ->.
+  move/ord_neq; rewrite eq_sym =>/negbTE -> /=.
+  by apply/permEl/perm_catl; rewrite perm_cons.
+move/negbT; rewrite !negb_or; case/and3P=>/negbTE Hxl /negbTE -> /negbTE Hxr;
+rewrite {}Hxl in Hl; rewrite {}Hxr in Hr.
+case: ifP=>/= H.
+- by rewrite -cat_cons; apply/permEl/perm_catr.
+rewrite -(cat1s x) -(cat1s a) -(cat1s a (inorder r)).
+rewrite perm_sym perm_catC -!catA catA perm_sym catA.
+apply/permEl/perm_catl; apply: (perm_trans Hr).
+by rewrite cats1 -perm_rcons.
+Qed.
+
+(* As a corollary, we can show that insertion preserves the tree invariant *)
+Lemma bst_insert x (t : tree T) : bst t -> bst (insert x t).
+Proof.
+elim: t=>//=l IHl a r IHr /and4P [Hal Har Hl Hr].
+case: ifP; first by move=>_ /=; rewrite Hal Har Hl Hr.
+move=>Hx; case: ifP=>Ho /=.
+- rewrite Har (IHl Hl) Hr /= andbT (perm_all _ (inorder_insert x Hl)).
+  by case: ifP=>//= _; rewrite Ho.
+rewrite Hal Hl (IHr Hr) /= andbT (perm_all _ (inorder_insert x Hr)).
+case: ifP=>//= _; rewrite Har andbT.
+by case: ordP=>//; [rewrite Ho| rewrite Hx].
+Qed.
+
+(* Insertion commutes on in-order representation *)
+Lemma insert_insert_perm x1 x2 (t : tree T) :
+        bst t ->
+        perm_eq (inorder (insert x1 (insert x2 t)))
+                (inorder (insert x2 (insert x1 t))).
+Proof.
+move=>H.
+have H1: (bst (insert x1 t)) by apply: bst_insert.
+have H2: (bst (insert x2 t)) by apply: bst_insert.
+apply: (perm_trans (inorder_insert x1 H2)); rewrite perm_sym.
+apply: (perm_trans (inorder_insert x2 H1)).
+move: (inorder_insert x1 H)=>{H1}Hi1.
+move: (inorder_insert x2 H)=>{H2}Hi2.
+rewrite (perm_mem Hi1 x2) (perm_mem Hi2 x1).
+case Hx1: (x1 \in inorder t); case Hx2: (x2 \in inorder t).
+- apply: (perm_trans Hi1); rewrite Hx1 perm_sym.
+  by apply: (perm_trans Hi2); rewrite Hx2.
+- rewrite inE Hx1 orbT perm_sym.
+  apply: (perm_trans Hi2); rewrite Hx2 perm_cons perm_sym.
+  by apply: (perm_trans Hi1); rewrite Hx1.
+- rewrite Hx1 inE Hx2 orbT.
+  apply: (perm_trans Hi1); rewrite Hx1 perm_cons perm_sym.
+  by apply: (perm_trans Hi2); rewrite Hx2.
+rewrite !inE Hx2 Hx1 !orbF; case: ifP.
+- by move/eqP=>->; rewrite eq_refl.
+rewrite eq_sym =>->.
+move: Hi1; rewrite -(perm_cons x2) Hx1=>H'; apply: (perm_trans H').
+rewrite -cat1s -(cat1s x1) perm_catCA /= perm_cons perm_sym.
+by apply: (perm_trans Hi2); rewrite Hx2.
+Qed.
+
+(* Moreover, such representations are equal *)
+Corollary insert_insert x1 x2 (t : tree T) :
+            bst t ->
+            inorder (insert x1 (insert x2 t)) = inorder (insert x2 (insert x1 t)).
+Proof.
+move=>H; apply: ord_sorted_eq.
+- by rewrite -bst_to_sorted; do 2!apply: bst_insert.
+- by rewrite -bst_to_sorted; do 2!apply: bst_insert.
+by apply/perm_mem/insert_insert_perm.
+Qed.
+
+(* Lookup in the tree is equivalent to lookup in the in-order *)
+Lemma inorder_search (t : tree T) :
+        bst t ->
+        search t =i inorder t.
+Proof.
+move=>+ x; elim: t=>//=l IHl a r IHr /and4P [Hal Har /IHl Hl /IHr Hr] {IHl IHr}.
+rewrite -topredE /= in Hl; rewrite -topredE /= in Hr.
+rewrite -topredE /= mem_cat inE {}Hl {}Hr.
+case: ifP=>_ /=; first by rewrite orbT.
+case: ifP=>Hx.
+- suff: x \notin inorder r by move/negbTE=>->/=; rewrite orbF.
+  by apply: (all_notin Har); apply/negP/nsym.
+suff: x \notin inorder l by move/negbTE=>->.
+by apply: (all_notin Hal)=>/=; rewrite Hx.
+Qed.
+
+(* Pointer-based procedures *)
+
+Opaque mknode.
+
+(* Inserting into the BST *)
+
+Definition inserttreeT x : Type :=
+  forall p,
+    {t : tree T}, STsep (shape p t,
+                        [vfun p' => shape p' (insert x t)]).
+
+Program Definition inserttree x : inserttreeT x :=
+  Fix (fun (go : inserttreeT x) p =>
+    Do (if p == null
+          then n <-- mknode x;
+               ret n
+          else a <-- !(p.+ 1);
+               if x == a then ret p
+                 else if ord x a
+                   then l <-- !p;
+                        l' <-- go l;
+                        p ::= l';;
+                        ret p
+                   else r <-- !(p.+ 2);
+                        r' <-- go r;
+                        p.+ 2 ::= r';;
+                        ret p)).
+Next Obligation.
+(* pull out ghost + precondition, branch on null check *)
+move=>x go p [t][] i /= H; case: eqP H=>[{p}->|/eqP E] H.
+- (* the tree is empty, make a new node *)
+  apply: vrfV=>V; case: (shape_null V H)=>{t H}->{i V}->.
+  by apply: [stepE]=>// n m H; step.
+(* the tree is a node, deconstruct it *)
+case: (shape_cont E H)=>l[z][r][pl][pr][_][{t H}->{i}->][hl][hr][-> Hl Hr].
+(* read the value, if the element is equal to it, just exit *)
+(* the tree shouldn't have duplicates *)
+step; case: eqP=>_; first by step; vauto.
+(* branch on comparison, read corresponding pointer *)
+case: ifP=>Ho; step.
+- (* insert in the left branch, update the left pointer *)
+  apply: [stepX l]@hl=>//= p' h' H'.
+  by do 2!step; vauto.
+(* insert in the right branch, update the right pointer *)
+apply: [stepX r]@hr=>//= p' h' H'.
+by do 2!step; vauto.
+Qed.
+
+(* Lookup in the BST *)
+
+(* lopp invariant: the tree is unchanged, return true if the element is found *)
+Definition searchtreeT x : Type :=
+  forall p,
+    {t : tree T}, STsep (shape p t,
+                        [vfun b h => shape p t h /\ b == search t x]).
+
+Program Definition searchtree x : searchtreeT x :=
+  Fix (fun (go : searchtreeT x) p =>
+    Do (if p == null
+          then ret false
+          else a <-- !(p.+ 1);
+               if x == a then ret true
+                 else if ord x a
+                   then l <-- !p;
+                        go l
+                   else r <-- !(p.+ 2);
+                        go r)).
+Next Obligation.
+(* pull out ghost + precondition, branch on null check *)
+move=>x go p [t][] i /= H; case: eqP H=>[{p}->|/eqP E] H.
+- (* tree is empty, it can't contain anything *)
+  by apply: vrfV=>V; case: (shape_null V H)=>{t H}->{i V}->; step.
+(* the tree is a node, deconstruct it *)
+case: (shape_cont E H)=>l[z][r][pl][pr][_][{t H}->{i}->][hl][hr][-> Hl Hr].
+(* read the value, compare it to the element, return true if it matches *)
+step; case: eqP=>_; first by step; vauto.
+(* branch on comparison, read corresponding pointer *)
+case: ifP=>Ho; step.
+- (* loop on the left branch *)
+  by apply: [gX l]@hl=>//= b h' [H' E'] _; vauto.
+(* loop on the right branch *)
+by apply: [gX r]@hr=>//= b h' [H' E'] _; vauto.
+Qed.
+
+(* test that the API is consistent, i.e. BST invariant is preserved *)
+(* and lookup finds previously inserted elements *)
+Program Definition test p x1 x2 :
+  {t : tree T}, STsep (fun h => shape p t h /\ bst t,
+                       [vfun (pb : ptr * bool) h =>
+                         let t' := insert x2 (insert x1 t) in
+                         [/\ shape pb.1 t' h, bst t' & pb.2]]) :=
+  Do (p1 <-- inserttree x1 p;
+      p2 <-- inserttree x2 p1;
+      b <-- searchtree x1 p2;
+      ret (p2, b)).
+Next Obligation.
+(* pull out ghost + precondition *)
+move=>p x1 x2 [t][] i /= [Ht Hi].
+(* run the subroutines, return the final tree and the lookup result *)
+apply: [stepE t]=>//= {p i Ht} p1 h1 H1.
+apply: [stepE (insert x1 t)]=>//= {p1 h1 H1} p2 h2 H2.
+apply: [stepE (insert x2 (insert x1 t))]=>//= {h2 H2} b h3 [H3 /eqP Hb].
+step=>_.
+(* insertions preserve the invariant *)
+have Hi2: bst (insert x2 t) by apply: bst_insert.
+have Hi21: bst (insert x2 (insert x1 t)) by do 2!apply: bst_insert.
+(* at this point we're done with the separation logic part, i.e. the mutable state *)
+(* the only non-trivial goal remaining is search being consistent with insert *)
+split=>//{p2 h3 H3}; rewrite {b}Hb.
+(* switch to in-order lookup *)
+move: (inorder_search Hi21 x1); rewrite -topredE /= =>->.
+(* use the insertion commutativity, unroll the insertion spec *)
+rewrite (insert_insert _ _ Hi) (perm_mem (inorder_insert x1 Hi2) x1).
+(* the goal is now trivially solved by case *)
+by case: ifP=>// _; rewrite inE eq_refl.
+Qed.
+
+End BST.
